cedar-dafny/validation/types.dfy
@@ -20,6 +20,16 @@ module validation.types {
   import opened def.base
   import opened def.core
 
+  // The ValidationMode determines whether to use permissive or strict typechecking
+  datatype ValidationMode = Permissive | Strict {
+    predicate isStrict() {
+      match this {
+        case Permissive => false
+        case Strict => true
+      }
+    }
+  }
+
   // --------- Types --------- //
 
   datatype BoolType = AnyBool | True | False {
@@ -56,8 +66,14 @@ module validation.types {
     function union(other: EntityLUB): EntityLUB {
       match (this, other) {
         case (EntityLUB(tys1),EntityLUB(tys2)) =>
-          // if either LUB contains an Action, then return AnyEntity
-          if exists ty1 <- tys1 :: isAction(ty1) || exists ty2 <- tys2 :: isAction(ty2)
+          // Check if either LUB contains an Action entity type. We do not
+          // permit any LUBs that contain different action entity types, so
+          // their union is `AnyEntity` if they are not the same action entity
+          // type. This also gives `AnyEntity` if they are the same action
+          // entity type, but some other entity types in the LUB differ. We
+          // never construct non-singleton action EntityLUBs, so this cannot
+          // occur.
+          if (exists ty1 <- tys1 :: isAction(ty1) || exists ty2 <- tys2 :: isAction(ty2)) && tys1 != tys2
           then AnyEntity
           else EntityLUB(tys1 + tys2)
         case _ => AnyEntity
@@ -86,6 +102,10 @@ module validation.types {
     predicate isOpen() {
       attrsTag.OpenAttributes?
     }
+
+    predicate isStrictType() {
+      forall k | k in attrs.Keys :: attrs[k].ty.isStrictType()
+    }
   }
 
   // Each extension function is associated with argument types, a return type,
@@ -101,6 +121,17 @@ module validation.types {
     Record(RecordType) |
     Entity(lub: EntityLUB) |
     Extension(Name)
+  {
+    predicate isStrictType() {
+      match this {
+        case Never => false
+        case String | Int | Bool(_) | Extension(_) => true
+        case Set(t) => t.isStrictType()
+        case Record(rt) => rt.isStrictType()
+        case Entity(lub) => lub.EntityLUB? && |lub.tys| == 1
+      }
+    }
+  }
 
   datatype SetStringType = SetType(Type) | StringType
   datatype RecordEntityType = Record(RecordType) | Entity(EntityLUB)
@@ -114,7 +145,11 @@ module validation.types {
     AttrNotFound(Type,Attr) |
     UnknownEntities(set<EntityType>) |
     ExtensionErr(Expr) |
-    EmptyLUB
+    EmptyLUB |
+    EmptySetForbidden |
+    NonLitExtConstructor |
+    NonSingletonLub |
+    HierarchyNotRespected
 
   // --------- Local Names for Useful Types --------- //
 
