cedar-dafny/validation/all.dfy
@@ -14,7 +14,6 @@
  * limitations under the License.
  */
 
-include "strict.dfy"
 include "subtyping.dfy"
 include "typechecker.dfy"
 include "types.dfy"
