cedar-dafny/validation/thm/strict_inf_strict.dfy
@@ -1,0 +1,172 @@
+/*
+ * Copyright 2022-2023 Amazon.com, Inc. or its affiliates. All Rights Reserved.
+ *
+ * Licensed under the Apache License, Version 2.0 (the "License");
+ * you may not use this file except in compliance with the License.
+ * You may obtain a copy of the License at
+ *
+ *      https://www.apache.org/licenses/LICENSE-2.0
+ *
+ * Unless required by applicable law or agreed to in writing, software
+ * distributed under the License is distributed on an "AS IS" BASIS,
+ * WITHOUT WARRANTIES OR CONDITIONS OF ANY KIND, either express or implied.
+ * See the License for the specific language governing permissions and
+ * limitations under the License.
+ */
+
+include "../../def/all.dfy"
+include "../all.dfy"
+include "base.dfy"
+include "model.dfy"
+include "soundness.dfy"
+
+// A quick proof checking that strict validation is reasonable.  Given a
+// strictly-type environment (see predicate `strictEnvironment`), the strict
+// typechecker should always infer a strict type (see `Type::isStrict()`) for
+// any expression assuming the expression is well typed.
+module validation.thm.strict_inf_strict {
+  import opened typechecker
+  import opened types
+  import opened subtyping
+  import opened base
+  import opened model
+  import opened soundness
+  import opened def.core
+  import opened def.engine
+  import opened ext
+
+  datatype StrictInfProof = StrictInfProof(
+    reqty: RequestType,
+    ets: EntityTypeStore,
+    acts: ActionStore
+  ) {
+
+    predicate strictEnvironment() {
+      reqty.principal.Some? &&
+      reqty.resource.Some? &&
+      reqty.context.isStrictType() &&
+      forall k | k in ets.types.Keys ::  ets.types[k].isStrictType()
+    }
+
+    const S_TC := Typechecker(ets,acts,reqty, ValidationMode.Strict)
+
+    lemma StrictRecord(e: Expr, r: seq<(Attr,Expr)>, effs: Effects)
+      decreases r
+      requires forall i | 0 <= i < |r| :: r[i] < e
+      requires strictEnvironment()
+      requires S_TC.inferRecord(e, r, effs).Ok?
+      ensures S_TC.inferRecord(e, r, effs).value.isStrictType()
+    {
+      reveal S_TC.inferRecord();
+      if r != [] {
+        assert S_TC.infer(r[0].1,effs).value.0.isStrictType() by {StrictTypeInf(r[0].1, effs); }
+        assert S_TC.inferRecord(e, r[1..], effs).value.isStrictType() by { StrictRecord(e, r[1..], effs); }
+      }
+    }
+
+    lemma StrictSetElems(e: Expr, es: seq<Expr>, effs: Effects)
+      decreases es
+      requires forall i | 0 <= i < |es| :: es[i] < e
+      requires strictEnvironment()
+      requires S_TC.inferSet(e, es, effs).Ok?
+      ensures es == [] ==> S_TC.inferSet(e, es, effs).value == Never
+      ensures  es != [] ==> S_TC.inferSet(e, es, effs).value.isStrictType()
+    {
+      if es != []  {
+        var (t,_) := S_TC.infer(es[0],effs).value;
+        assert t.isStrictType() by { StrictTypeInf(es[0], effs); }
+        var t1 := S_TC.inferSet(e,es[1..],effs).value;
+        assert t1.isStrictType() || t1 == Never by { StrictSetElems(e, es[1..], effs); }
+        var t2 := lubOpt(t,t1,ValidationMode.Strict).value;
+        assert t2.isStrictType() by { StrictTypeLub(t, t1); }
+      }
+    }
+
+    lemma StrictIf(g: Expr, t: Expr, e: Expr, effs: Effects)
+      decreases If(g, t, e), 0
+      requires strictEnvironment()
+      requires S_TC.infer(If(g, t, e), effs).Ok?
+      ensures S_TC.infer(If(g, t, e), effs).value.0.isStrictType()
+    {
+      var (bt,effs1) := S_TC.inferBoolType(g,effs).value;
+      match bt {
+        case True =>
+          var (t1,effs2) := S_TC.infer(t,effs.union(effs1)).value;
+          StrictTypeInf(t, effs.union(effs1));
+        case False =>
+          var (t2,effs2) := S_TC.infer(e,effs).value;
+          StrictTypeInf(e, effs);
+        case Bool =>
+          var (t1,effs2) := S_TC.infer(t,effs.union(effs1)).value;
+          var (t2,effs3) := S_TC.infer(e,effs).value;
+          StrictTypeInf(t, effs.union(effs1));
+          StrictTypeInf(e, effs);
+          StrictTypeLub(t1, t2);
+      }
+    }
+
+    lemma StrictGetAttr(e: Expr, l: Attr, effs:Effects)
+      decreases GetAttr(e, l), 0
+      requires strictEnvironment()
+      requires S_TC.infer(GetAttr(e, l), effs).Ok?
+      ensures S_TC.infer(GetAttr(e, l), effs).value.0.isStrictType()
+    {
+      assert S_TC.inferRecordEntityType(e,effs).Ok?;
+      StrictTypeInf(e, effs);
+    }
+
+    lemma StrictHasAttr(e: Expr, l: Attr, effs: Effects)
+      decreases HasAttr(e, l), 0
+      requires strictEnvironment()
+      requires S_TC.infer(HasAttr(e, l), effs).Ok?
+      ensures S_TC.infer(HasAttr(e, l), effs).value.0.isStrictType()
+    { }
+
+    lemma StrictIn(e1: Expr, e2: Expr, effs: Effects)
+      decreases BinaryApp(BinaryOp.In, e1, e2), 0
+      requires strictEnvironment()
+      requires S_TC.infer(BinaryApp(BinaryOp.In, e1, e2), effs).Ok?
+      ensures S_TC.infer(BinaryApp(BinaryOp.In, e1, e2), effs).value.0.isStrictType()
+    { }
+
+    lemma StrictCall(name: base.Name, args: seq<Expr>, effs: Effects)
+      decreases args
+      requires strictEnvironment()
+      requires S_TC.infer(Call(name, args), effs).Ok?
+      ensures S_TC.infer(Call(name, args), effs).value.0.isStrictType()
+    { }
+
+    lemma StrictTypeInf(e: Expr, effs: Effects)
+      decreases e, 1
+      requires strictEnvironment()
+      requires S_TC.infer(e, effs).Ok?
+      ensures S_TC.infer(e, effs).value.0.isStrictType()
+    {
+      match e {
+        case PrimitiveLit(p) =>
+        case Var(x) =>
+        case If(e',e1,e2) => StrictIf(e', e1, e2, effs);
+        case And(e1,e2) =>
+        case Or(e1,e2) =>
+        case UnaryApp(Not,e') =>
+        case UnaryApp(Neg,e') =>
+        case UnaryApp(MulBy(i),e') =>
+        case UnaryApp(Like(p),e') =>
+        case BinaryApp(Eq,e1,e2) =>
+        case BinaryApp(Less,e1,e2) =>
+        case BinaryApp(LessEq,e1,e2) =>
+        case BinaryApp(Add,e1,e2) =>
+        case BinaryApp(Sub,e1,e2) =>
+        case BinaryApp(In,e1,e2) => StrictIn(e1, e2, effs);
+        case BinaryApp(ContainsAny,e1,e2) =>
+        case BinaryApp(ContainsAll,e1,e2) =>
+        case BinaryApp(Contains,e1,e2) =>
+        case Record(es) => StrictRecord(e, es, effs);
+        case Set(es) => StrictSetElems(e, es, effs);
+        case GetAttr(e',l) => StrictGetAttr(e', l, effs);
+        case HasAttr(e',l) => StrictHasAttr(e', l, effs);
+        case Call(name,es) => StrictCall(name, es, effs);
+      }
+    }
+  }
+}
